intermediate/Veritas.Intermediate.Thread.fsti
@@ -1,9 +1,66 @@
 module Veritas.Intermediate.Thread
 
-open Veritas.Intermediate.Logs
-open Veritas.Intermediate.VerifierConfig
-open Veritas.Intermediate.Store
-
+open Veritas.BinTree
 open Veritas.MultiSetHashDomain
+open Veritas.Record
+open Veritas.SeqAux
+open Veritas.Intermediate.Logs
+open Veritas.Intermediate.Store
+open Veritas.Intermediate.Verify
+open Veritas.Intermediate.VerifierConfig
+
+module SA = Veritas.SeqAux
+module IntV = Veritas.Intermediate.Verify
 
 let thread_id_logS vcfg = thread_id & logS vcfg
+
+let thread_id_of #vcfg (tl: thread_id_logS vcfg): nat = fst tl
+
+let logS_of #vcfg (tl: thread_id_logS vcfg): logS _ = snd tl
+
+let length #vcfg (tl: thread_id_logS vcfg): nat =
+  Seq.length (logS_of tl)
+
+let tl_idx #vcfg (tl: thread_id_logS vcfg) = i:nat{i < length tl}
+
+let index #vcfg (tl: thread_id_logS vcfg) (i:tl_idx tl): logS_entry _ =
+  Seq.index (logS_of tl) i
+
+let prefix #vcfg (tl: thread_id_logS vcfg) (i:nat{i <= length tl}): thread_id_logS _ =
+  (thread_id_of tl), (SA.prefix (logS_of tl) i)
+
+let init_store vcfg (tid:thread_id): vstore _ = 
+  let st = empty_store vcfg in
+  if tid = 0 then 
+    madd_to_store_root st 0 (init_value Root) 
+  else
+    st
+
+val lemma_init_store_ismap (vcfg:verifier_config) (tid:thread_id)
+  : Lemma (ensures (is_map (init_store vcfg tid)))
+          [SMTPat (init_store vcfg tid)]
+
+val lemma_init_store_slot_points_to_is_merkle_points_to (vcfg:verifier_config) (tid:thread_id)
+  : Lemma (ensures (slot_points_to_is_merkle_points_to (init_store vcfg tid)))
+          [SMTPat (init_store vcfg tid)]
+
+let verify #vcfg (tl:thread_id_logS vcfg): vtls _ =
+  let (tid,l) = tl in
+  let st = init_store vcfg tid in
+  let vs = IntV.init_thread_state tid st in
+  IntV.verify vs l
+
+let verifiable #vcfg (tl:thread_id_logS vcfg) = 
+  IntV.Valid? (verify tl)
+
+let verifiable_log vcfg = tl:thread_id_logS vcfg{verifiable tl}
+
+val verifiable_implies_prefix_verifiable
+  (#vcfg:_) (tl:verifiable_log vcfg) (i:nat{i <= length tl}):
+  Lemma (ensures (verifiable (prefix tl i)))
+        [SMTPat (prefix tl i)]
+
+(* clock after processing the i'th entry *)
+let clock #vcfg (tl:verifiable_log vcfg) (i:tl_idx tl): timestamp =
+  let vs = verify (prefix tl (i + 1)) in
+  Valid?.clock (verify (prefix tl (i + 1)))
