intermediate/Veritas.Intermediate.Correctness.fst
@@ -1,0 +1,16 @@
+module Veritas.Intermediate.Correctness
+
+open Veritas.State
+open Veritas.Verifier.EAC
+open Veritas.Intermediate.Global
+open Veritas.Intermediate.Thread
+open Veritas.Intermediate.VerifierConfig
+
+module IntG = Veritas.Intermediate.Global
+
+// final correctness property
+let lemma_verifier_correct (#vcfg:_) (gl: hash_verifiable_log vcfg { ~ (seq_consistent (IntG.to_state_ops gl))})
+  : hash_collision_gen = 
+  (* sequences of per-thread put/get operations *)
+  let g_ops = IntG.to_state_ops gl in
+  admit()
