intermediate/Veritas.Intermediate.Global.fsti
@@ -1,0 +1,37 @@
+module Veritas.Intermediate.Global
+
+open FStar.Seq
+open Veritas.MultiSetHashDomain
+open Veritas.SeqAux
+open Veritas.Intermediate.Logs
+open Veritas.Intermediate.Thread
+
+module SA = Veritas.SeqAux
+module IntLog = Veritas.Intermediate.Logs
+module IntT = Veritas.Intermediate.Thread
+
+let g_logS vcfg = seq (logS vcfg)
+
+let thread_log #vcfg (gl:g_logS vcfg) (tid:seq_index gl): thread_id_logS _ = 
+   (tid, Seq.index gl tid)
+
+let to_state_ops #vcfg (gl:g_logS vcfg) =
+  map IntLog.to_state_ops gl
+
+let verifiable #vcfg (gl: g_logS vcfg) = 
+  forall (tid:seq_index gl). {:pattern IntT.verifiable (thread_log gl tid)} IntT.verifiable (thread_log gl tid)
+
+let verifiable_log vcfg = gl:g_logS vcfg{verifiable gl}
+
+val verifiable_implies_prefix_verifiable
+  (#vcfg:_) (gl:verifiable_log vcfg) (i:nat{i <= Seq.length gl}):
+  Lemma (ensures (verifiable #vcfg (SA.prefix gl i)))
+        [SMTPat (SA.prefix gl i)]
+
+val hadd (#vcfg:_) (gl: verifiable_log vcfg): ms_hash_value
+val hevict (#vcfg:_) (gl: verifiable_log vcfg): ms_hash_value
+
+let hash_verifiable #vcfg (gl: verifiable_log vcfg): bool = 
+  hadd gl = hevict gl
+
+let hash_verifiable_log vcfg = gl:verifiable_log vcfg{hash_verifiable gl}
