intermediate/Veritas.Intermediate.TSLog.fsti
@@ -1,0 +1,19 @@
+module Veritas.Intermediate.TSLog
+
+open Veritas.Interleave
+open Veritas.State
+open Veritas.Intermediate.Global
+open Veritas.Intermediate.Logs
+
+module IntL = Veritas.Intermediate.Logs
+
+let il_logS vcfg = interleaving (logS_entry vcfg)
+
+let thread_count #vcfg (il:il_logS vcfg) = Seq.length (s_seq il)
+
+let valid_tid #vcfg (il:il_logS vcfg) = tid:nat{tid < thread_count il}
+
+let g_logS_of #vcfg (il:il_logS vcfg): g_logS _ = s_seq il
+
+let to_state_ops #vcfg (itsl:il_logS vcfg): Seq.seq (state_op) =
+  IntL.to_state_ops (i_seq itsl)
